
\section{Proofs} \label{s:proofs}

\subsection{Theorem \ref{thm: Steenrod-Adem on Barratt-Eccles}}

We prove that the $\Z[\mathrm{C}_r]$-linear map
\begin{equation*}
\psi_{\mathcal E}(r) : \mathcal W(r) \to \mathcal E(r)
\end{equation*}
introduced in Definition \ref{def: Steenrod-Adem on Barratt-Eccles} is a chain map for every $r \geq 0$. We simplify notation and write $\psi$ instead of $\psi_{\mathcal E}(r)$. To show $\psi$ is a chain map we proceed by induction. Notice that
\begin{equation*}
\psi(\partial e_0) = 0 = \partial \psi(e_0)
\end{equation*}
and assume $\psi(\partial e_{k-1}) = \partial \psi(e_{k-1})$. If $k = 2n$ we have
\begin{align*}
\partial \psi(e_{2n}) & = 
\partial \sum_{r_1, \dots, r_n} 
\big(\rho^0, \rho^{r_1}, \rho^{r_1+1}, \dots, \rho^{r_n}, \rho^{r_n+1} \big)  \\ & =
\partial \sum_{r_2, \dots, r_n} \sum_{r_1 = 0}^{p-1}
\big(\rho^0, \rho^{r_1} \, (\rho^0, \rho^{1}, \dots, \rho^{r_n-r_1}, \rho^{r_n - r_1 +1}) \big) \\ & =
\partial \sum_{r_2, \dots, r_n}
\big(\rho^0, N\, (\rho^{0}, \rho^{1}, \dots, \rho^{r_n}, \rho^{r_n + 1}) \big) \\ & =
\sum_{r_2, \dots, r_n}
N\, \big( \rho^{0}, \rho^{1}, \dots, \rho^{r_n}, \rho^{r_n + 1} \big) \\ & -
\sum_{r_2, \dots, r_n}
\big(\rho^0, \partial \, N \, (\rho^{0}, \rho^{1}, \dots, \rho^{r_n}, \rho^{r_n+1}) \big) \\ & =
N \psi(e_{2n-1}) - (\rho^0, \partial N \psi (e_{2n-1})) \\ & =
\psi(N e_{2n-1}) - (\rho^0, \psi (\partial N e_{2n-1})) \\ & =
\psi(\partial e_{2n}) - (\rho^0, \psi (\partial^2 e_{2n})) \\ & =
\psi(\partial e_{2n}).
\end{align*}
If $k = 2n+1$ we have
\begin{align*}
\partial \psi(e_{2n+1}) & = 
\partial \sum_{r_1, \dots, r_n} 
\big(\rho^0, \rho^1, \rho^{r_1}, \rho^{r_1+1}, \dots, \rho^{r_n}, \rho^{r_n+1} \big)  \\ & =
\partial \sum_{r_1, \dots, r_n}
\big(\rho^0, \rho^{1} \, (\rho^0, \rho^{r_1-1}, \rho^{r_1}, \dots, \rho^{r_n - 1}, \rho^{r_n}) \big) \\ & =
\partial \sum_{r_1, \dots, r_n}
\big(\rho^0, T\, (\rho^0, \rho^{r_1-1}, \rho^{r_1}, \dots, \rho^{r_n - 1}, \rho^{r_n}) \big) \\ & =
\sum_{r_1, \dots, r_n}
T \, \big( \rho^0, \rho^{r_1-1}, \rho^{r_1}, \dots, \rho^{r_n - 1}, \rho^{r_n} \big) \\ & -
\sum_{r_1, \dots, r_n}
\big(\rho^0, \partial \, T \, (\rho^0, \rho^{r_1-1}, \rho^{r_1}, \dots, \rho^{r_n - 1}, \rho^{r_n}) \big) \\ & =
T \psi(e_{2n}) - (\rho^0, \partial T \psi (e_{2n})) \\ & =
\psi(T e_{2n}) - (\rho^0, \psi (\partial T e_{2n})) \\ & =
\psi(\partial e_{2n+1}) - (\rho^0, \psi (\partial^2 e_{2n+1})) \\ & =
\psi(\partial e_{2n+1})
\end{align*}
where for the third equality we used that for any $r_1, \dots, r_n$
\begin{equation*}
(\rho^0, \rho^0, \rho^{r_1-1}, \rho^{r_1}, \dots, \rho^{r_n - 1}, \rho^{r_n}) = 0.
\end{equation*}
This map is a quasi-isomorphism since both complexes have the homology of a point and $\psi(e_0)$ represents a generator of the homology.

\subsection{Theorem \ref{thm: Steenrod-Adem on surjection MS convention}}

\begin{proof}
	We prove that the $\Z[\mathrm{C}_r]$-linear map
	\begin{equation*}
	\psi_{\mathcal X}(r) : \mathcal W(r) \to \mathcal X(r)
	\end{equation*}
	introduced in Definition \ref{def: Steenrod-Adem on surjection} is a chain map for every $r \geq 0$. We simplify notation and write $\psi$ instead of $\psi_{\mathcal X}(r)$. To show $\psi$ is a chain map we proceed by induction. Notice that
	\begin{equation*}
	\psi(\partial e_0) = 0 = \partial \psi(e_0)
	\end{equation*}
	and assume $\psi(\partial e_{n-1}) = \partial \psi(e_{n-1})$. For $n = 2m+1$ we have
	\begin{align*}
	\partial \psi(e_{2m+1}) 
	& =
	\partial\, h\, T\, \psi(e_{2m}) \big) \\
	& =
	T\, \psi(e_{2m}) - i^{r-1} p^{r-1}\, \psi(e_{2m}) -
	h\, \partial\, T\, \psi(e_{2m}) \big) \\
	& =
	T\, \psi(e_{2m}) - 
	h\, T\, \psi(\partial\, e_{2m}) \big) \\
	& =
	T\, \psi(e_{2m}) - 
	h\, \psi(T\,N\, e_{2m-1}) \big) \\
	& = 
	T \psi(e_{2m}).
	\end{align*}
	For $n = 2m$ the proof is analogous. The chain map $\psi$ is a quasi-isomorphism since both complexes have the homology of a point and $\psi(e_0) = (1, \dots, r)$ is a generator of the homology.
\end{proof}

\subsection{Theorem \ref{thm: cubical chain bialgebra}}

The only non-trivial relation we need to verify is
\begin{equation*}
\partial \product = \, \boundary \, .
\end{equation*}
Let us consider two basis elements of $N_\bullet(\square^n) = N_\bullet(\square^1)^{\otimes n}$
\begin{align*}
x & = x_1 \otimes \cdots \otimes x_n, \\
y & = y_1 \otimes \cdots \otimes y_n.
\end{align*}
We need to show that
\begin{equation*}
\partial (x \ast y) + \partial x \ast y + (-1)^{|x|}x \ast \partial y = \epsilon(x) y - \epsilon(y) x.
\end{equation*}
We have
\begin{equation*}
x \ast y = \sum (-1)^{|x|} \epsilon(y_{<i})x_{<i} \otimes x_i \ast y_i \otimes \epsilon(x_{>i})y_{>i}
\end{equation*}
and
\begin{align*}
\partial(x \ast y) & = 
\sum (-1)^{|x|} \epsilon(y_{<i}) \partial x_{<i} \otimes x_i \ast y_i \otimes \epsilon(x_{>i}) y_{>i} \\ & +
\sum (-1)^{|x|+|x_{<i}|} \epsilon(y_{<i}) x_{<i} \otimes \partial (x_i \ast y_i) \otimes \epsilon(x_{>i}) y_{>i} \\ & -
\sum (-1)^{|x|+|x_{<i}|} \epsilon(y_{<i}) x_{<i} \otimes x_i \ast y_i \otimes \epsilon(x_{>i}) \partial y_{>i}.
\end{align*}
Since
\begin{equation*}
|x| = |x_{<i}| + |x_i| + |x_{>i}|, \quad \epsilon(x_{>i}) \neq 0 \Leftrightarrow |x_{>i}| = 0, \quad \partial(x_i \ast y_i) \neq 0 \Rightarrow |x_i| = 0,
\end{equation*}
we have
\begin{equation} \label{eq: boundary of product 1}
\begin{split}
\partial(x \ast y) & = 
\sum (-1)^{|x|} \epsilon(y_{<i}) \partial x_{<i} \otimes x_i \ast y_i \otimes \epsilon(x_{>i}) y_{>i} \\ & +
\sum \epsilon(y_{<i}) x_{<i} \otimes \partial (x_i \ast y_i) \otimes \epsilon(x_{>i}) y_{>i} \\ & -
\sum \epsilon(y_{<i}) x_{<i} \otimes x_i \ast y_i \otimes \epsilon(x_{>i}) \partial y_{>i}.
\end{split}
\end{equation}
We also have
\begin{align*}
\partial x \ast y & = 
\sum (-1)^{|x|-1} \epsilon(y_{<i}) \partial x_{<i} \otimes x_i \ast y_i \otimes \epsilon(x_{>i}) y_{>i} \\ & +
\sum (-1)^{|x|-1+|x_{<i}|} \epsilon(y_{<i}) x_{<i} \otimes \partial x_i \ast y_i \otimes \epsilon(x_{>i}) y_{>i} \\ & +
\sum (-1)^{|x|-1+|x_{<i}|} \epsilon(y_{<i}) x_{<i} \otimes x_i \ast y_i \otimes \epsilon(\partial x_{>i}) y_{>i}.
\end{align*}
Since
\begin{equation*}
\epsilon(\partial x_{>i}) = 0, \quad \partial x_i \neq 0 \Leftrightarrow |x_i| = 1,
\end{equation*}
we have
\begin{equation} \label{eq: boundary of product 2}
\begin{split}
\partial x \ast y & = 
\sum (-1)^{|x|-1} \epsilon(y_{<i}) \partial x_{<i} \otimes x_i \ast y_i \otimes \epsilon(x_{>i}) y_{>i} \\ & +
\sum \epsilon(y_{<i}) x_{<i} \otimes \partial x_i \ast y_i \otimes \epsilon(x_{>i}) y_{>i}.
\end{split}
\end{equation}
We also have
\begin{align*}
(-1)^{|x|} x \ast \partial y & = 
\sum \epsilon(\partial y_{<i}) x_{<i} \otimes x_i \ast y_i \otimes \epsilon(x_{>i}) y_{>i} \\ & +
\sum (-1)^{|y_{<i}|} \epsilon(y_{<i}) x_{<i} \otimes x_i \ast \partial y_i \otimes \epsilon(x_{>i}) y_{>i} \\ & +
\sum (-1)^{|y_{<i}|+|y_i|} \epsilon(y_{<i}) x_{<i} \otimes x_i \ast y_i \otimes \epsilon(x_{>i}) \partial y_{>i},
\end{align*}
which is equivalent to
\begin{equation} \label{eq: boundary of product 3}
\begin{split}
(-1)^{|x|} x \ast \partial y & = 
\sum \epsilon(y_{<i}) x_{<i} \otimes x_i \ast \partial y_i \otimes \epsilon(x_{>i}) y_{>i} \\ & +
\sum \epsilon(y_{<i}) x_{<i} \otimes x_i \ast y_i \otimes \epsilon(x_{>i}) \partial y_{>i}.
\end{split}
\end{equation}
Putting identities \eqref{eq: boundary of product 1}, \eqref{eq: boundary of product 2} and \eqref{eq: boundary of product 3} together, we get
\begin{multline*}
\partial (x \otimes y) + \partial x \ast y + (-1)^{|x|}x \ast \partial y =
\sum \epsilon(y_{<i}) x_{<i} \otimes \big(\partial(x_i \ast y_i) + \partial x_i \ast y_i + x_i \ast \partial y_i\big) \otimes \epsilon(x_{>i}) y_{>i}.
\end{multline*}
Since
\begin{equation*}
\partial(x_i \ast y_i) + \partial x_i \ast y_i + x_i \ast \partial y_i = \epsilon(x_i)y_i - \epsilon(y_i)x_i,
\end{equation*}
we have
\begin{align*}
\partial (x \ast y) + \partial x \ast y + & (-1)^{|x|}x \ast \partial y \\ = &
\sum \epsilon(y_{<i}) x_{<i} \otimes \epsilon(x_{\geq i}) y_{\geq i} - \epsilon(y_{\leq i}) x_{\leq i} \otimes \epsilon(x_{>i}) y_{>i} \\ = &
\epsilon(x)y - \epsilon(y)x,
\end{align*}
as desired, where the last equality follows from a telescopic sum argument.